Slightly slicker proof in callrec

src/x86/callrec.v
@@ -36,25 +36,6 @@ Definition call_toyfun f :=
 Definition mkbody_toyfun (p: program) :=
   p;; popcode ;; JMP retreg.
 
-(* It's useful to define local functions *)
-Notation "'let_toyfun' f  ':=' p 'in' q" :=
-  (LOCAL skip; JMP skip;; LOCAL f; f:;; mkbody_toyfun p;; skip:;; q)%asm
-  (at level 45, f ident, right associativity).
-
-
-(* Example recursive function *)
-Definition toyfun_example_recursivecallee : program :=
-  mkbody_toyfun (
-  LOCAL L; LOCAL SKIP;
-  L:;;
-    INC EBX;;
-    DEC EAX;;
-    JZ SKIP;;
-    call_toyfun L;;
-  SKIP:;
-  )%asm.
-
-
 Lemma spec_at_toyfun f P Q R:
   toyfun f P Q @ R -|- toyfun f (P**R) (Q**R).
 Proof.
@@ -66,47 +47,6 @@ Proof.
 Qed.
 Hint Rewrite spec_at_toyfun : push_at.
 
-Lemma basic_seq_frame (c1 c2: program) S P Q R F:
-  S |-- basic P c1 Q @ F ->
-  S |-- basic Q c2 R @ F ->
-  S |-- basic P (c1;; c2) R @ F.
-Proof.
-  move=> Hc1 Hc2. rewrite spec_at_basic. eapply basic_seq. 
-  rewrite ->spec_at_basic in Hc1. apply Hc1.  
-  rewrite ->spec_at_basic in Hc2. apply Hc2.  
-Qed.  
-
-Lemma basic_local_frame S P c Q R:
-  (forall l, S |-- (basic P (c l) Q @ R)) ->
-  S |-- basic P (prog_declabel c) Q @ R.
-Proof.
-  rewrite ->spec_at_basic. move => H. apply basic_local => l. specialize (H l). by rewrite ->spec_at_basic in H.  
-Qed. 
-
-Lemma toyfun_call (f:DWORD) P Q vs:
-  |> toyfun f P Q |-- basic P (call_toyfun f) Q @ (retreg? ** stackinv vs).
-Proof.
-  rewrite /call_toyfun. 
-  apply basic_local_frame => iret. 
-  rewrite -spec_at_at spec_at_swap spec_at_basic. 
-  apply: basic_seq_frame. 
-  basic apply pushaxiom. 
-  rewrite /basic. specintros => i j. unfold_program. specintros => *; do !subst.
-
-  rewrite spec_at_swap. rewrite spec_at_impl. 
-  superspecapply *.
-
-  rewrite <- (spec_frame (i -- iret :-> JMP f)). rewrite /toyfun. autorewrite with push_at.
-  apply limplAdj. apply landAdj.
-  
-  autorewrite with push_later; last apply _. 
-  rewrite spec_at_later.
-  autorewrite with push_later. eapply lforallL.
-  autorewrite with push_later; last apply _. autorewrite with push_at. eapply lforallL.   
-  autorewrite with push_at. autorewrite with push_later; last apply _.
-  cancel2. rewrite <- spec_later_weaken. finish_logic_with sbazooka. finish_logic_with sbazooka. 
-Qed.
-
 Lemma toyfun_call_recAux (f:DWORD) P Q vs (i j:DWORD):
   |-- (|> toyfun f P Q -->> (safe @ (EIP ~= j ** Q) -->> safe @ (EIP ~= i ** P)) @ (retreg? ** stackinv vs)) @ (i -- j :-> call_toyfun f).
 Proof. rewrite /call_toyfun. unfold_program. 
@@ -117,17 +57,20 @@ Proof. rewrite /call_toyfun. unfold_program.
   autorewrite with push_at. 
   autorewrite with push_later; last apply _. eapply lforallL.
 
-  superspecapply pushaxiom.
-  superspecapply JMP_I_rule. autorewrite with push_at. 
+  (* pushcode *)
+  superspecapply *. 
+  (* JMP f *)
+  superspecapply *. 
+  autorewrite with push_at. 
   autorewrite with push_later; last apply _.
   cancel2.
-  rewrite <- spec_later_weaken. cancel1. sbazooka.
-  cancel1. sbazooka. 
+  rewrite <- spec_later_weaken. finish_logic_with sbazooka. 
+  finish_logic_with sbazooka. 
 Qed.
 
 Corollary toyfun_call_rec (f:DWORD) P Q R vs (i j:DWORD):
  |> toyfun f P Q @ (i -- j :-> call_toyfun f ** R)  |-- (safe @ (EIP ~= j ** Q) -->> safe @ (EIP ~= i ** P)) @ (retreg? ** stackinv vs) @ (i -- j :-> call_toyfun f ** R).
-Proof.
+Proof. 
 apply limplValid. rewrite <- spec_at_later. rewrite <- spec_at_impl. 
 rewrite <-spec_at_at. rewrite <- spec_frame. apply toyfun_call_recAux. 
 Qed. 
@@ -151,189 +94,118 @@ Proof.
   finish_logic_with sbazooka.  
 Qed.
 
-(* the following shows we didn't need that stackinv in there above (could have framed it anyway)
-   not immediately clear to me which version one actually wants
-*)
-Lemma toyfun_mkbody' (f f': DWORD) P p Q:
-  basic (P) p (Q)  |--
-    toyfun f P Q @ (f--f' :-> mkbody_toyfun p).
-Proof.
-  rewrite /toyfun. specintro => iret. rewrite /mkbody_toyfun.
-  unfold_program. specintros => i1 i' vs.
-   
-  autorewrite with push_at. 
-  apply limplAdj. 
-  eapply (safe_safe_context _); first reflexivity. apply landL1.
-  do 2 eapply lforallL. reflexivity. 
-  by ssimpl.  
-
-  superspecapply *.
-  superspecapply *. rewrite <-spec_later_weaken. 
-  finish_logic_with sbazooka. 
-Qed.
-
 Lemma lobentails S : (|> S -->> S) |-- S.
 apply spec_lob_context.
 apply landAdj; reflexivity.
 Qed.
 
 (* now playing with recursion *)
-Lemma lobunderAt (f:DWORD) P Q p f' : (|-- (|> toyfun f P Q -->> toyfun f P Q) @ (f -- f' :-> mkbody_toyfun p)) -> (|-- toyfun f P Q @ (f -- f' :-> mkbody_toyfun p)).
-move => H.
-apply spec_lob_context. apply landL2. apply limplValid. autorewrite with push_at in H. 
-autorewrite with push_at. assumption. 
-Qed.
+Definition weakenContext (P Q:spec) : |-- Q -> P |-- Q.
+Proof. move => H. by rewrite <- H. Qed. 
 
-Lemma rocov S S' R : S |-- S' -> S @ R |-- S' @ R.
-move => H.
-rewrite <-H.
-reflexivity.
-Qed.
+(* Example recursive function, with instructions nailed down *)
+Definition exSpec f := Forall a b, toyfun f (EAX ~= a ** EBX ~= b) (EAX ~= #0 ** EBX ~= addB b a) @ OSZCP?.
 
-(* arggh, different levels of entailment are really vexing *)
-Lemma lobunderAt' (f:DWORD) P Q p f' : ((|> toyfun f P Q -->> toyfun f P Q) @ (f -- f' :-> mkbody_toyfun p)) |-- (toyfun f P Q @ (f -- f' :-> mkbody_toyfun p)).
-apply rocov.
-apply lobentails.
-Qed.
+(* Example recursive function *)
+Definition toyfun_example_recursivecallee_program : program :=
+  mkbody_toyfun (
+  LOCAL L; LOCAL SKIP;
+  L:;;
+    INC EBX;;
+    DEC EAX;;
+    JZ SKIP;;
+    call_toyfun L;;
+  SKIP:;
+  )%asm.
 
-(* possibly an easier way to do that! *)
-
-Lemma toyfun_mkbody_context S (f f': DWORD) P p Q:
-  S //\\ basic P p Q  |--
-  (S -->>  toyfun f P Q) @ (f--f' :-> mkbody_toyfun p).
+Theorem toyfun_example_correct_program (i1 i2:DWORD) :
+  |-- exSpec i1 @ (i1 -- i2 :-> toyfun_example_recursivecallee_program).
 Proof.
-  rewrite /toyfun. specintro => iret. rewrite /mkbody_toyfun. 
-  unfold_program. autorewrite with push_at.
-  specintros => vs i1 i'.
+rewrite /toyfun_example_recursivecallee_program/mkbody_toyfun.
 
-  apply limplAdj. autorewrite with push_at.  
-  apply limplAdj. 
-  eapply (safe_safe_context _); first reflexivity. apply landL1. apply landL1.
-  apply landL2. do 2 eapply lforallL. reflexivity. 
+(* Do this BEFORE applying spec_lob or you will get in a mess with existentials *)
+unfold_program. 
+specintros => i3 i4 i5 i6 <- <- i7 i8 i9 i10 <- <- i11. 
+(* Cleanup *)
+rewrite empSPR empSPL 3!sepSPA. 
+
+(* Now apply the Lob rule *)
+apply spec_lob.
+
+rewrite {2}/exSpec/toyfun. 
+specintros => a b iret vs. 
+
+(* Push non-code bit of frame inside *)
+do 2 rewrite spec_at_impl. 
+
+(* Pull out arbitrary flags and register *)
+rewrite {7 8 9 10 11 12}/stateIsAny.
+specintros => o s z c p r. simpl in o,s,z,c,p,a,r.
+
+(* We want these unfolded in the rules *)
+Hint Unfold OSZCP ConditionIs : specapply. 
+
+(* INC EBX *)
+superspecapply *. 
+
+(* DEC EAX *)
+superspecapply *. 
+
+(* JZ SKIP *)
+superspecapply *. 
+
+specsplit. 
+- (* Would be nice if we had a reflective tactic that did this *)
+  setoid_rewrite <- spec_later_weaken at 2.
+  specintros => /eqP/eqP EQ.  
+  (* popcode *)
+  specapply *. rewrite /stateIsAny. sbazooka.     
+  (* JMP retreg *)
+  superspecapply *. 
+  (* usual stuff; should be able to automate this a bit *)
+  apply weakenContext. rewrite <- spec_frame. apply limplValid. rewrite <- spec_later_weaken. 
+  autorewrite with push_at. cancel1. rewrite /stateIsAny. sbazooka.  
+  (* Arithmetic *)
+  rewrite -{2}(decBK a). rewrite EQ incB_fromNat addB1. 
   by ssimpl. 
 
-  superspecapply *.
-  superspecapply *. rewrite <- spec_later_weaken.
-  finish_logic_with sbazooka. 
-Qed.
-
-
-
-(* Now, as a special case of the above, we can define singly-recursive functions 
-   But note that this actual form of definition is rarely going to be useful as it
-   bakes in a particular P and Q, which will only be any use for trivial functions - we'll
-   usually want some quantification and adaptation in there
-*)
-Lemma toyfun_mkbody_rec (f f': DWORD) P p Q:
-  |> toyfun f P Q //\\ basic P p Q  |--
-  (toyfun f P Q) @ (f--f' :-> mkbody_toyfun p).
-Proof.
-rewrite <-lobunderAt'. apply toyfun_mkbody_context.  
-Qed.
-
-(*
-   Example that shows a caller and a callee independently verified and then
-   composed.
- *)
-
-Definition exSpec f := Forall a b, toyfun f (EAX ~= a ** EBX ~= b) (EAX ~= #0 ** EBX ~= addB b a) @ OSZCP?.
-Example toyfun_example_body_correct (f f': DWORD):
-  |-- (|> exSpec f -->> exSpec f) @ (f -- f' :-> toyfun_example_recursivecallee).
-Proof.  
-  rewrite /toyfun_example_recursivecallee/mkbody_toyfun. (*unfold_program.*)
-  rewrite {2}/exSpec. 
-  specintros => a b. 
-  rewrite /toyfun.
-  specintros => iret vs.
-  rewrite spec_at_impl. 
-  rewrite spec_at_impl.
-  rewrite spec_at_impl. 
-
-(*  specintro => i1. specintro => i2 i3 i4 <- <- i5 i6 i7 i8 <- <- i9. *)
-  rewrite /stateIsAny.
-  specintros => o s z c p r.
-  simpl in o,s,z,c,p,a,r.
-
-  apply limplValid. 
-
-  (* Why do we need this? Answer: because specapply doesn't unfold stuff in rules in contrast to basic apply  *)
-  (* INC EBX *)
-  unfold_program. unfold_program.
-  specintros => i1 i2 i3 i4 <- <- i5 i6 i7 i8 <- <- i9.
-  instrrule pose (INC_R_rule (r:=EBX)) as RULE.
-  rewrite /OSZCP in RULE. rewrite spec_at_at. 
-  superspecapply RULE. clear RULE.
-
-  (* DEC EAX *)
-  instLem (DEC_R_rule (r:=EAX)) => RULE. 
-  rewrite /OSZCP in RULE.
-  superspecapply RULE. clear RULE. 
-
-  (* JZ SKIP *)
-  superspecapply JZ_rule. 
-  specsplit. 
-  - setoid_rewrite <- spec_later_weaken at 2. specintros => H.
-    specapply popaxiom. 
-      rewrite /stateIsAny. sbazooka. 
-    superspecapply *. setoid_rewrite <- spec_later_weaken at 2. 
-    autorewrite with push_at.
-    finish_logic. apply landL2. cancel1. sbazooka.
-    rewrite -{2}(decBK a).  
-    rewrite (eqP (eqP H)). rewrite incB_fromNat addB1. by ssimpl. 
-
- - specintros => H. rewrite (eqP H).  
-   rewrite /exSpec. 
+- specintros => /eqP ->. 
+  rewrite /exSpec. 
+  (* All this just to instantiate quantifiers on left of turnstile *)
      autorewrite with push_later; last apply _. rewrite spec_at_forall. apply lforallL with (decB a).
      autorewrite with push_later; last apply _. rewrite spec_at_forall. apply lforallL with (incB b).
      rewrite spec_at_toyfun.
-   set PRE := (EAX ~= decB _ ** _) ** _. 
    rewrite  -addB_decB_incB  decBK incBK.  
+   
+   set PRE := (EAX ~= decB _ ** _) ** _. 
    set POST := (EAX ~= #0 ** _) ** _.       
-   
-   set I1 := (f -- i5 :-> _). 
-   set I2 := (i5 -- i6 :-> _). 
-   set I3 := (i6 -- i7 :-> _). 
-   set I4 := (i8 -- i9 :-> _). 
-   set I5 := (i9 -- f' :-> _). 
-   instLem (@toyfun_call_rec f (PRE) (POST) (I1**I2**I3**I4**I5)) => TFC.
-   unfold I1, I2, I3, I4, I5 in *.
+   instLem (@toyfun_call_rec i1 PRE POST (i1 -- i7 :-> (INC EBX)%asm**i7 -- i8 :-> (DEC EAX)%asm**i8 -- i9 :-> JZ%asm i10**i10 -- i11 :-> popcode**i11 -- i2 :-> JMP retreg)) => TFC. 
 
-   
    (* call_toyfun L *)
    (* Have to rearrange in order to get frame right *)
-(*   rewrite -> (spec_at_swap _ (_ -- _ :-> call_toyfun f)) in TFC. *)
-   rewrite -> spec_at_impl in TFC. 
-   do 2 rewrite -> (spec_at_at safe) in TFC.
    rewrite /toyfun in TFC.
-   (* But now we do at least get to use specapply *)
-   specapply TFC; last first.
+   rewrite -> spec_at_impl in TFC.
+   repeat rewrite ->(spec_at_at safe) in TFC.
+   repeat rewrite -> (spec_at_at safe).
+   rewrite /toyfun.
+   rewrite spec_at_later.
+      
+   eapply (safe_safe_frame1 _).
+   exact TFC. cancel1. specintros => iret' vs'. 
+   rewrite spec_at_forall. apply lforallL with iret'. 
+   rewrite spec_at_forall. apply lforallL with vs'. autorewrite with push_at. 
+   cancel2. cancel1. sbazooka. cancel1. sbazooka.
+   rewrite /ConditionIs/PRE/stateIsAny. split. sbazooka. sbazooka.
 
+   apply weakenContext. rewrite {TFC}. 
    (* popcode *)
    rewrite /PRE/POST.
-   superspecapply popaxiom. 
+   superspecapply *. 
    (* JMP retreg *)
    superspecapply *. 
    (* Usual logic stuff *)
-   setoid_rewrite <- spec_later_weaken at 2. autorewrite with push_at. 
-   apply limplAdj. apply landL2. 
-   rewrite /POST/stateIsAny. cancel1. sbazooka. 
-   rewrite /PRE/stateIsAny. sbazooka.
-
-
-   (* Now the remaining obligation from specapply TFC. *)
-   autorewrite with push_later; last apply _. rewrite /toyfun. 
-   autorewrite with push_at. specintros => iret'. 
-   autorewrite with push_at. cancel1. 
-   specintros => vs'. apply lforallL with iret'. rewrite spec_at_forall. 
-   apply lforallL with vs'. 
-   rewrite spec_at_at. rewrite spec_at_at.
-   autorewrite with push_at. cancel2. cancel1. admit.  cancel1. sbazooka. 
+   setoid_rewrite <- spec_later_weaken. 
+   rewrite /POST/PRE/stateIsAny. 
+   finish_logic_with sbazooka.
 Qed.
-
-Corollary toyfun_example_correct (f f': DWORD):
-  |-- exSpec f @ (f--f' :-> toyfun_example_recursivecallee).
-Proof.
-apply spec_lob. apply limplValid. rewrite <-spec_at_later. 
-rewrite <- spec_at_impl. apply toyfun_example_body_correct. 
-Qed. 
 
